\documentclass[15pt,landscape]{article}
\usepackage{amsmath,amssymb,amsfonts,amsthm}
\usepackage[german]{babel}
\usepackage[utf8]{inputenc}
\usepackage{fancyhdr}
%\usepackage[a3paper]{geometry}
\usepackage{geometry}
\usepackage{tikz}
\usepackage{xcolor}
\usetikzlibrary{automata,positioning}
\geometry{top=20mm, left=20mm, right=10mm, bottom=15mm}


\newcommand{\hr}{\begin{center} \line(1,0){450} \end{center}}
\newcommand{\R}{\mathbb R}
\newcommand{\tr}{^\mathsf{T}}
\newcommand{\F}{\mathcal{F}}
\newcommand{\norm}[1]{\left\lVert#1\right\rVert}
\DeclareMathOperator{\Id}{Id}
\DeclareMathOperator{\diag}{diag}
\DeclareMathOperator{\epi}{epi}
\DeclareMathOperator{\co}{co}
\DeclareMathOperator{\interior}{int}
\DeclareMathOperator{\Proj}{Pr}
\DeclareMathOperator*{\argmin}{argmin}
\DeclareMathOperator*{\argmax}{argmax}
\newcommand{\midd}{\mathrel{}\middle|\mathrel{}}


\pagestyle{fancy}
\lhead{Christian Lengert}
\rhead{\today}
\chead{153767}
%\rfoot{Page \thepage}

\begin{document}

\begin{center}
	\section*{Konvexe Optimierung}
	\subsection*{Projekt}
\end{center}
\hr
\subsubsection*{$L_1$ Loss}
\newcommand{\oneLossReg}{\max \left\{ 0,1-y_i \cdot \left( w\tr x_i + b \right) \right\}}
\begin{equation}
\min\limits_{w,b} f_1(x) = \frac{1}{2} w\tr w +c \cdot \sum\limits_{i=1}^k \left[ \oneLossReg \right]
\end{equation}
\paragraph{Dual Form}

\begin{align}
\max\limits_{\alpha} \min\limits_{w,b} f_1^\alpha(x) &= \frac{1}{2} w\tr w +c \cdot \sum\limits_{i=1}^k \alpha_i \left[ \oneLossReg \right] \nonumber \\
&= \frac{1}{2} w\tr w +c \cdot \sum\limits_{i=1}^k \alpha_i \left(  1-y_i \cdot \left( w\tr x_i + b \right) \right)\\
\end{align}


\begin{align}
\frac{\partial}{\partial w} f^{\alpha}_3(x) &= \frac{\partial}{\partial w} \left[  \frac{1}{2} w\tr w +c \cdot \sum\limits_{i=1}^k \alpha_i \left[ \oneLossReg \right] \right]\nonumber\\
&= \frac{\partial}{\partial w} \left[  \frac{1}{2} w\tr w \right] + \frac{\partial}{\partial w} \left[  c \cdot \sum\limits_{i=1}^k \alpha_i \left[\oneLossReg \right] \right]\nonumber\\
&= w +   c \cdot \sum\limits_{i=1}^k \alpha_i \frac{\partial}{\partial w} \left[\oneLossReg \right]\nonumber\\
&= w +   c \cdot \sum\limits_{i=1}^k \alpha_i \frac{\partial}{\partial w} \left[1-y_i \cdot \left( w\tr x_i + b \right) \right]\nonumber\\
&= w +   c \cdot \sum\limits_{i=1}^k \alpha_i \frac{\partial}{\partial w} \left[1-y_i \cdot \left( w\tr x_i + b \right) \right]\nonumber\\
&= w +   c \cdot \sum\limits_{i=1}^k \alpha_i \frac{\partial}{\partial w} \left[-y_i \cdot \left( w\tr x_i + b \right) \right]\nonumber\\
&= w +   c \cdot \sum\limits_{i=1}^k \alpha_i \frac{\partial}{\partial w} \left[\left( -y_i w\tr x_i + -y_i b \right) \right]\nonumber\\
&= w +   c \cdot \sum\limits_{i=1}^k \alpha_i \frac{\partial}{\partial w} \left[ -y_i w\tr x_i + -y_i b \right]\nonumber\\
&= w -   c \cdot \sum\limits_{i=1}^k \alpha_i  y_i x_i \nonumber\\
&\Rightarrow w =  c \cdot \sum\limits_{i=1}^k \alpha_i y_i x_i\label{df1w}
\end{align}

\begin{align*}
\frac{\partial}{\partial b} f^{\alpha}_3(x) &= \frac{\partial}{\partial b} \left[  \frac{1}{2} w\tr w +c \cdot \sum\limits_{i=1}^k \alpha_i \left[ \oneLossReg \right] \right]\\
&= \frac{\partial}{\partial b} \left[  c \cdot \sum\limits_{i=1}^k \alpha_i \left[ \oneLossReg \right] \right]\\
&=   c \cdot \sum\limits_{i=1}^k \alpha_i \frac{\partial}{\partial b} \left[  \oneLossReg \right]\\
&=   c \cdot \sum\limits_{i=1}^k \alpha_i \frac{\partial}{\partial b} \left[  1-y_i \cdot \left( w\tr x_i + b \right) \right]\\
&=   c \cdot \sum\limits_{i=1}^k \alpha_i \frac{\partial}{\partial b} \left[ -y_i \cdot \left( w\tr x_i + b \right) \right]\\
&=   c \cdot \sum\limits_{i=1}^k \alpha_i -y_i\\
&\Rightarrow 0 =    c \cdot \sum\limits_{i=1}^k \alpha_i y_i\\
\end{align*}


\begin{align}
f_1^\alpha(x) &= \frac{1}{2} w\tr w +c \cdot \sum\limits_{i=1}^k \alpha_i \left[ \oneLossReg \right] \nonumber \\
&= \frac{1}{2} w\tr w +c \cdot \sum\limits_{i=1}^k \alpha_i \left(  1-y_i \cdot \left( w\tr x_i + b \right) \right)\\
&\stackrel{\eqref{df1w}}{\Rightarrow} \frac{1}{2} \left( c \cdot \sum\limits_{i=1}^k \alpha_i  y_i x_i \right)\tr \left( c \cdot \sum\limits_{i=1}^k \alpha_i  y_i x_i \right) +c \cdot \sum\limits_{i=1}^k \alpha_i \left(  1-y_i \cdot \left( \left( c \cdot \sum\limits_{j=1}^k \alpha_j  y_j x_j \right)\tr x_i + b \right) \right)\\
&= \frac{1}{2} \left( c \cdot \sum\limits_{i=1}^k \alpha_i  y_i x_i \right)\tr \left( c \cdot \sum\limits_{i=1}^k \alpha_i  y_i x_i \right) +c \cdot \sum\limits_{i=1}^k \alpha_i \left(  1- \left( c \cdot \sum\limits_{j=1}^k \alpha_j y_i  y_j x_j\tr x_i \right)  \right)\\
&= \frac{1}{2} \left( c \cdot \sum\limits_{i=1}^k \alpha_i  y_i x_i \right)\tr \left( c \cdot \sum\limits_{i=1}^k \alpha_i  y_i x_i \right) +c \cdot \sum\limits_{i=1}^k \left(  \alpha_i  -  \left( c \cdot \sum\limits_{j=1}^k \alpha_i \alpha_j y_i  y_j x_j\tr x_i \right)  \right)\\
&= \frac{1}{2} \left( c \cdot \sum\limits_{i=1}^k \alpha_i  y_i x_i \right)\tr \left( c \cdot \sum\limits_{i=1}^k \alpha_i  y_i x_i \right) +c \cdot \sum\limits_{i=1}^k   \alpha_i  - c \cdot   \sum\limits_{i=1}^k \sum\limits_{j=1}^k \alpha_i \alpha_j y_i  y_j x_j\tr x_i \\
&= \frac{1}{2} \left( c \cdot \sum\limits_{i=1}^k \alpha_i  y_i x_i \right)\tr \left( c \cdot \sum\limits_{i=1}^k \alpha_i  y_i x_i \right) +c \cdot \sum\limits_{i=1}^k   \alpha_i  - c \cdot \left(  \left(\sum\limits_{i=1}^k \alpha_i  y_i x_i \right)\tr \left(\sum\limits_{i=1}^k \alpha_i  y_i x_i \right) \right) \\
&= c \cdot \sum\limits_{i=1}^k   \alpha_i  - c \cdot \frac{1}{2} \sum\limits_{i=1}^k \sum\limits_{j=1}^k \alpha_i \alpha_j y_i  y_j x_j\tr x_i \\
\end{align}


\hr
\subsubsection*{$L_2$ Loss}
\begin{equation}
\min\limits_{w,b} f_2(x) = \frac{1}{2} w\tr w +c \cdot \sum\limits_{i=1}^k \left[ \max \left\{ 0,1-y_i \cdot \left( w\tr x_i + b \right) \right\}^2\right]
\end{equation}
\newcommand{\twoLossReg}{\max \left\{ 0,1-y_i \cdot \left( w\tr x_i + b \right)\right\}^2 }

\paragraph{Dual Form}
\begin{align*}
\max\limits_{\alpha} \min\limits_{w,b} f^{\alpha}_2(x) = \frac{1}{2} w\tr w +c \cdot \sum\limits_{i=1}^k \alpha_i \left[ \twoLossReg \right]\\
\end{align*}

\begin{align}
\frac{\partial}{\partial w} f^{\alpha}_2(x) &= \frac{\partial}{\partial w} \left[  \frac{1}{2} w\tr w +c \cdot \sum\limits_{i=1}^k \alpha_i \left[ \twoLossReg \right] \right]\nonumber\\
&= \frac{\partial}{\partial w} \left[  \frac{1}{2} w\tr w \right] + \frac{\partial}{\partial w} \left[  c \cdot \sum\limits_{i=1}^k \alpha_i \left[\twoLossReg \right] \right]\nonumber\\
&= w +   c \cdot \sum\limits_{i=1}^k \alpha_i \frac{\partial}{\partial w} \left[\twoLossReg \right]\nonumber\\
&= w +   c \cdot \sum\limits_{i=1}^k \alpha_i \frac{\partial}{\partial w} \left[  \left(1-y_i \cdot \left( w\tr x_i + b \right) \right)^2 \right]\nonumber\\
&= w +   c \cdot \sum\limits_{i=1}^k \alpha_i \frac{\partial}{\partial w} \left[ 1 - 2 \left(y_i \cdot \left( w\tr x_i + b \right) \right) + y_i^2 \cdot \left( w\tr x_i + b \right)^2 \right]\nonumber\\
&= w +   c \cdot \sum\limits_{i=1}^k \alpha_i \frac{\partial}{\partial w} \left[ 1 - 2 y_i w\tr x_i - 2 y_i b  + y_i^2 w\tr w x_i^2 + y_i^2 2 w\tr x_i  b + y_i^2 b^2 \right]\nonumber\\
&= w +   c \cdot \sum\limits_{i=1}^k \alpha_i 2 y_i x_i   + 2 y_i^2 w\tr x_i^2 + y_i^2 2 w\tr x_i  b \nonumber\\
\end{align}



\hr
\subsubsection*{Logistic Loss}
\newcommand{\zLog}{1+\exp(-y_i (w\tr x_i + b))}

\begin{equation}
\min\limits_{w,b} f_3(x) = \frac{1}{2} w\tr w +c \cdot \sum\limits_{i=1}^k \left[ \ln(\zLog)\right]\\
\end{equation}

\paragraph{Dual Form}
\begin{align*}
\max\limits_{\alpha} \min\limits_{w,b} f^{\alpha}_3(x) = \frac{1}{2} w\tr w +c \cdot \sum\limits_{i=1}^k \alpha_i \left[ \ln(\zLog)\right]\\
\end{align*}

\begin{align*}
\frac{\partial}{\partial w} f^{\alpha}_3(x) &= \frac{\partial}{\partial w} \left[  \frac{1}{2} w\tr w +c \cdot \sum\limits_{i=1}^k \alpha_i \left[ \ln(\zLog)\right] \right]\\
&= \frac{\partial}{\partial w} \left[  \frac{1}{2} w\tr w \right] + \frac{\partial}{\partial w} \left[  c \cdot \sum\limits_{i=1}^k \alpha_i \left[\ln(\zLog)\right] \right]\\
&=  w  +  c \cdot \sum\limits_{i=1}^k \frac{\partial}{\partial w} \left[  \alpha_i \left[\ln(\zLog)\right] \right]\\
&=  w  +  c \cdot \sum\limits_{i=1}^k \frac{\partial}{\partial w} \left[  \alpha_i \left[\ln(\zLog)\right] \right]\\
&=  w  +  c \cdot \sum\limits_{i=1}^k \alpha_i  \frac{\partial}{\partial w}  \left[\ln(\zLog)\right] \\
&=  w  +  c \cdot \sum\limits_{i=1}^k \alpha_i  \frac{ -y_i w\exp(-y_i(w\tr x_i + b)) }{\zLog}\\
\end{align*}


%\begin{align*}
%\frac{\partial}{\partial w} f_3(x) &= \frac{\partial}{\partial w} \left[ \frac{1}{2} w\tr w \right] +c \cdot \sum\limits_{i=1}^k \frac{\partial}{\partial w} \left[ \ln(\zLog)\right]\\
%&= w +c \cdot \sum\limits_{i=1}^k \frac{\partial}{\partial w} \left[ \ln(\zLog)\right]\\
%\end{align*}

%\begin{align*}
%\frac{\partial}{\partial x} f_3(x) &= \frac{\partial}{\partial x} \frac{1}{2} w\tr w +c \cdot \sum\limits_{i=1}^k \frac{\partial}{\partial x} \left[ \ln(\zLog)\right]\\
%&= c \cdot \sum\limits_{i=1}^k \frac{\partial}{\partial x} \left[ \ln(1+\exp(-y_i\left(w\tr x_i + b \right) ))\right] \\
%&= c \cdot \sum\limits_{i=1}^k \frac{\frac{\partial}{\partial x} \left[ 1+\exp(-y_i(w\tr x_i + b)) \right]} {\zLog} \\
%&= c \cdot \sum\limits_{i=1}^k \frac{\frac{\partial}{\partial x} \left[ \exp(-y_i(w\tr x_i + b))\right]}{\zLog} \\
%&= c \cdot \sum\limits_{i=1}^k \frac{ \exp(-y_i(w\tr x_i + b)) \frac{\partial}{\partial x} \left[ -y_i (w\tr x_i + b)  \right]}{\zLog}\\
%&= c \cdot \sum\limits_{i=1}^k \frac{ \exp(-y_i(w\tr x_i + b)) \frac{\partial}{\partial x} \left[ -y_i w\tr x_i -y_i b \right]}{\zLog}\\
%&= c \cdot \sum\limits_{i=1}^k \frac{ -y_i w\exp(-y_i(w\tr x_i + b)) }{\zLog}\\
%%&= c \cdot \sum\limits_{i=1}^k \frac{ -y_i w\exp(-y_i(w^{(1)} x^{(1)}_i + w^{(2)} x^{(2)}_i + b)) }{\zLog}\\
%\end{align*}
%
%\newcommand{\dLogz}{-y_i w \exp(-y_i(w\tr x_i + b))}
%\newcommand{\dLogn}{\zLog}


%\begin{align*}
%\frac{\partial}{\partial x \partial x} f_3(x) &= \frac{\partial}{\partial x}\left[ c \cdot \sum\limits_{i=1}^k \frac{\dLogz}{\dLogn}  \right] \\
%&= c \cdot \sum\limits_{i=1}^k \frac{\partial}{\partial x} \left[  \frac{\dLogz}{\dLogn}  \right] = c \cdot \sum\limits_{i=1}^k \frac{ \frac{\partial}{\partial x} u(x_i) \cdot v(x_i) - u(x_i) \cdot \frac{\partial}{\partial x_i} v(x_i)} {v(x_i)^2}\\
%\end{align*}

%\begin{align*}
%u(x) &= \dLogz\\
%v(x) &= \dLogn\\
%\frac{\partial}{\partial x} u(x) &= \frac{\partial}{\partial x} \left[\dLogz \right]\\
% &= -y_i w \exp(-y_i(w\tr x_i + b)) \frac{\partial}{\partial x} \left[ -y_i(w\tr x_i + b) \right] \\
%&= y_i^2 w^2 \exp(-y_i(w\tr x_i + b)) \\  
%\frac{\partial}{\partial x}  v(x) &= \frac{\partial}{\partial x} \left[  \dLogn \right] \\ 
%&= \frac{\partial}{\partial x} \left[\exp(-y_i\left(w\tr x_i + b \right)) \right] \\ 
%&= u(x)
%\end{align*}
%
%\begin{align*}
%\frac{\partial}{\partial x \partial x} f_3(x) &= \frac{ y_i^2 w^2 \exp(-y_i(w\tr x_i + b)) \cdot \left(\dLogn\right) - \left( \dLogz \right)^2 } {\left(\dLogn\right)^2}\\
%\end{align*}



%&\text{with } u(x) = \dLogz \text{ and } v(x) = \dLogn \\
%u

%&= c \cdot \sum\limits_{i=1}^k \frac{\frac{\partial}{\partial x} \left[ \dLogz \right] \cdot \dLogn - \dLogz \cdot \frac{\partial}{\partial x} \left[ \dLogn \right] } {\dLogn^2}
%\end{align*}
\end{document}
