\documentclass[12pt,landscape]{article}
\usepackage{amsmath,amssymb,amsfonts,amsthm}
\usepackage[german]{babel}
\usepackage[utf8]{inputenc}
\usepackage{fancyhdr}
\usepackage[a3paper]{geometry}
\usepackage{tikz}
\usepackage{xcolor}
\usetikzlibrary{automata,positioning}
\geometry{top=20mm, left=20mm, right=10mm, bottom=15mm}


\newcommand{\hr}{\begin{center} \line(1,0){450} \end{center}}
\newcommand{\R}{\mathbb R}
\newcommand{\tr}{^\mathsf{T}}
\newcommand{\F}{\mathcal{F}}
\newcommand{\norm}[1]{\left\lVert#1\right\rVert}
\DeclareMathOperator{\Id}{Id}
\DeclareMathOperator{\diag}{diag}
\DeclareMathOperator{\epi}{epi}
\DeclareMathOperator{\co}{co}
\DeclareMathOperator{\interior}{int}
\DeclareMathOperator{\Proj}{Pr}
\DeclareMathOperator*{\argmin}{argmin}
\DeclareMathOperator*{\argmax}{argmax}
\newcommand{\midd}{\mathrel{}\middle|\mathrel{}}



\pagestyle{fancy}
\lhead{Christian Lengert}
\rhead{\today}
\chead{153767}
%\rfoot{Page \thepage}

\begin{document}

\begin{center}
	\section*{Konvexe Optimierung}
	\subsection*{Projekt}
\end{center}
\hr
%\subsubsection*{$L_1$ Loss}
%\begin{equation}
%\min\limits_{x \in \mathbb{R}^n} f_1(x) = \frac{1}{2} w\tr w +c \cdot \sum\limits_{i=1}^k \left[ \max \left\{ 0,1-y_i \cdot \left( w\tr x_i + b \right) \right\}\right]
%\end{equation}
%
%\begin{align}
%\frac{\partial}{\partial w} f_1(x) &= w + c \cdot \sum\limits_{i=1}^k  \frac{\partial}{\partial w} \left[ 1-y_i \cdot \left( w\tr x_i + b \right) \right]\\
%&= w + c \cdot \sum\limits_{i=1}^k  \frac{\partial}{\partial w} \left[ -y_i \cdot \left( w\tr x_i + b \right) \right]\\
%&= w + c \cdot \sum\limits_{i=1}^k  \frac{\partial}{\partial w} \left[ -y_iw\tr x_i + -y_ib \right]\\
%&= w + c \cdot \sum\limits_{i=1}^k  -y_i x_i \\
%\end{align}
%
%\begin{align}
%\frac{\partial}{\partial b} f_1(x) &= c \cdot \sum\limits_{i=1}^k  \frac{\partial}{\partial b} \left[ 1-y_i \cdot \left( w\tr x_i + b \right) \right]\\
%&= c \cdot \sum\limits_{i=1}^k  \frac{\partial}{\partial b} \left[ -y_i w\tr x_i + -y_ib \right]\\
%&= c \cdot \sum\limits_{i=1}^k  -y_i\\
%\end{align}
%
%\hr
\subsubsection*{$L_1$ Loss}
\begin{equation}
\min\limits_{x \in \mathbb{R}^n} f_1(x) = \frac{1}{2} \left(  w_1^2 + w_2^2 \right) +c \cdot \sum\limits_{i=1}^k \left[ \max \left\{ 0,1-y_i \cdot \left( w_1  x_1^{(i)} +  w_2  x_2^{(i)} + b \right) \right\}\right]
\end{equation}

\begin{align}
\frac{\partial}{\partial w_1} f_1(x) &= \frac{\partial}{\partial w_1}\frac{1}{2} \left[ w_1^2 + w_2^2 \right] + c \cdot \sum\limits_{i=1}^k  \frac{\partial}{\partial w_1} \left[ 1-y_i \cdot \left( w_1  x_1^{(i)} +  w_2  x_2^{(i)} + b \right) \right]\\
&= \frac{1}{2} 2w_1 + c \cdot \sum\limits_{i=1}^k  \frac{\partial}{\partial w_1} \left[ -y_i w_1  x_1^{(i)} -y_i  w_2  x_2^{(i)}  -y_ib \right]\\
&= w_1 - c \cdot \sum\limits_{i=1}^k y_i  x_1^{(i)}\\
\end{align}
\newcommand{\lOneLossDwOne}{w_1 - c \cdot \sum\limits_{i=1}^k y_i  x_1^{(i)}}

\begin{align}
\frac{\partial}{\partial w_2} f_1(x) &= w_2  - c \cdot \sum\limits_{i=1}^k y_i  x_2^{(i)} \\
\end{align}

\newcommand{\lOneLossDwTwo}{w_2  - c \cdot \sum\limits_{i=1}^k y_i  x_2^{(i)} }

\begin{align}
\frac{\partial}{\partial b} f_1(x) &= c \cdot \sum\limits_{i=1}^k  \frac{\partial}{\partial b} \left[ 1-y_i \cdot \left( w_1  x_1^{(i)} + w_2  x_2^{(i)} + b \right) \right]\\
&= c \cdot \sum\limits_{i=1}^k  \frac{\partial}{\partial b} \left[ -y_i w_1  x_1^{(i)} +  w_2  x_2^{(i)} -y_ib \right]\\
&= - c \cdot \sum\limits_{i=1}^k y_i\\
\end{align}


\begin{equation}
\mathcal{H}(f_1) = \begin{bmatrix}
\frac{\partial^2}{\partial w_1 \partial w_1} & \frac{\partial^2}{\partial w_1 \partial w_2} & \frac{\partial^2}{\partial w_1 \partial b}\\
\frac{\partial^2}{\partial w_2 \partial w_1} & \frac{\partial^2}{\partial w_2 \partial w_2} & \frac{\partial^2}{\partial w_2 \partial b}\\
\frac{\partial^2}{\partial b \partial w_1} & \frac{\partial^2}{\partial b \partial w_2} & \frac{\partial^2}{\partial b \partial b}\\
\end{bmatrix}
\end{equation}



\begin{align}
\frac{\partial^2}{\partial w_1 \partial w_1} &=  \frac{\partial}{\partial w_1} \left[  \lOneLossDwOne \right]  = \frac{\partial}{\partial w_1} \left[ w_1 \right] = 1
\end{align}

\begin{align}
\frac{\partial^2}{\partial w_1 \partial w_2} &=  \frac{\partial}{\partial w_2} \left[  \lOneLossDwOne \right] =  0
\end{align}

\begin{align}
\frac{\partial^2}{\partial w_1 \partial b} &=  \frac{\partial}{\partial b} \left[  \lOneLossDwOne \right] = 0
\end{align}

\begin{align}
\frac{\partial^2}{\partial w_2 \partial w_1} &=  \frac{\partial}{\partial w_1} \left[ \lOneLossDwTwo \right] = 0
\end{align}

\begin{align}
\frac{\partial^2}{\partial w_2 \partial w_2} &= \frac{\partial}{\partial w_2} \left[ \lOneLossDwTwo \right] = \frac{\partial}{\partial w_2} \left[ w_2 \right] = 1
\end{align}

\begin{align}
\frac{\partial^2}{\partial w_2 \partial w_1 b} &= \frac{\partial}{\partial b} \left[ \lOneLossDwTwo \right] = 0
\end{align}

\begin{align}
\frac{\partial^2}{\partial b \partial w_1} &= \frac{\partial}{\partial w_1} \left[  - c \cdot \sum\limits_{i=1}^k y_i \right] = 0
\end{align}

\begin{align}
\frac{\partial^2}{\partial b \partial w_2}  &= \frac{\partial}{\partial w_2} \left[  - c \cdot \sum\limits_{i=1}^k y_i \right] = 0
\end{align}

\begin{align}
\frac{\partial^2}{\partial b \partial b} &= \frac{\partial}{\partial b} \left[  - c \cdot \sum\limits_{i=1}^k y_i \right] = 0
\end{align}


\begin{equation}
\Rightarrow \mathcal{H}(f_1) = \begin{bmatrix}
1 & 0 & 0\\
0 & 1 & 0\\
0&0&0\\
\end{bmatrix}
\end{equation}


\hr
\subsubsection*{$L_2$ Loss}
\newcommand{\lTwoLoss}{1-y_i \cdot \left( w_1  x_1^{(i)} + w_2  x_2^{(i)} + b\right)}
\begin{equation}
\min\limits_{x \in \mathbb{R}^n} f_2(x) = \frac{1}{2} w_1^2 + w_2^2 +c \cdot \sum\limits_{i=1}^k \left[ \max \left\{ 0,\lTwoLoss  \right\}^2\right]
\end{equation}


\begin{align}
\frac{\partial}{\partial w_1} f_1(x) &= \frac{1}{2} \frac{\partial}{\partial w_1} \left[  w_1^2 + w_2^2 \right]  +c \cdot \sum\limits_{i=1}^k  \left[ \left( \lTwoLoss \right)^2 \right]\\
&= \frac{1}{2} \frac{\partial}{\partial w_1} \left[  w_1^2 + w_2^2 \right]  +c \cdot \sum\limits_{i=1}^k  \left[ \left( \lTwoLoss \right)^2 \right]
\end{align}

\begin{align}
\frac{\partial}{\partial w_2} f_1(x) &= w_1^2 + 2w_2  - c \cdot \sum\limits_{i=1}^k y_i  x_2^{(i)} \\
\end{align}



\begin{align}
\frac{\partial}{\partial b} f_1(x) &= c \cdot \sum\limits_{i=1}^k  \frac{\partial}{\partial b} \left[ 1-y_i \cdot \left( w_1  x_1^{(i)} + w_2  x_2^{(i)} + b \right) \right]\\
&= c \cdot \sum\limits_{i=1}^k  \frac{\partial}{\partial b} \left[ -y_i w_1  x_1^{(i)} +  w_2  x_2^{(i)} -y_ib \right]\\
&= - c \cdot \sum\limits_{i=1}^k y_i\\
\end{align}


\begin{equation}
\mathcal{H}(f_1) = \begin{bmatrix}
\frac{\partial^2}{\partial w_1 \partial w_1} & \frac{\partial^2}{\partial w_1 \partial w_2} & \frac{\partial^2}{\partial w_1 \partial b}\\
\frac{\partial^2}{\partial w_2 \partial w_1} & \frac{\partial^2}{\partial w_2 \partial w_2} & \frac{\partial^2}{\partial w_2 \partial b}\\
\frac{\partial^2}{\partial b \partial w_1} & \frac{\partial^2}{\partial b \partial w_2} & \frac{\partial^2}{\partial b \partial b}\\
\end{bmatrix}
\end{equation}







\hr
\subsubsection*{Logistic Loss}
\newcommand{\zLog}{1+\exp(-y_i (w\tr x_i + b))}

\begin{equation}
\min\limits_{x \in \mathbb{R}^n} f_3(x) = \frac{1}{2} w\tr w +c \cdot \sum\limits_{i=1}^k \left[ \ln(\zLog)\right]\\
\end{equation}

\begin{align*}
\frac{\partial}{\partial w} f_3(x) &= \frac{\partial}{\partial w} \left[ \frac{1}{2} w\tr w \right] +c \cdot \sum\limits_{i=1}^k \frac{\partial}{\partial w} \left[ \ln(\zLog)\right]\\
&= w +c \cdot \sum\limits_{i=1}^k \frac{\partial}{\partial w} \left[ \ln(\zLog)\right]\\
\end{align*}

\begin{align*}
\frac{\partial}{\partial x} f_3(x) &= \frac{\partial}{\partial x} \frac{1}{2} w\tr w +c \cdot \sum\limits_{i=1}^k \frac{\partial}{\partial x} \left[ \ln(\zLog)\right]\\
&= c \cdot \sum\limits_{i=1}^k \frac{\partial}{\partial x} \left[ \ln(1+\exp(-y_i\left(w\tr x_i + b \right) ))\right] \\
&= c \cdot \sum\limits_{i=1}^k \frac{\frac{\partial}{\partial x} \left[ 1+\exp(-y_i(w\tr x_i + b)) \right]} {\zLog} \\
&= c \cdot \sum\limits_{i=1}^k \frac{\frac{\partial}{\partial x} \left[ \exp(-y_i(w\tr x_i + b))\right]}{\zLog} \\
&= c \cdot \sum\limits_{i=1}^k \frac{ \exp(-y_i(w\tr x_i + b)) \frac{\partial}{\partial x} \left[ -y_i (w\tr x_i + b)  \right]}{\zLog}\\
&= c \cdot \sum\limits_{i=1}^k \frac{ \exp(-y_i(w\tr x_i + b)) \frac{\partial}{\partial x} \left[ -y_i w\tr x_i -y_i b \right]}{\zLog}\\
&= c \cdot \sum\limits_{i=1}^k \frac{ -y_i w\exp(-y_i(w\tr x_i + b)) }{\zLog}\\
%&= c \cdot \sum\limits_{i=1}^k \frac{ -y_i w\exp(-y_i(w^{(1)} x^{(1)}_i + w^{(2)} x^{(2)}_i + b)) }{\zLog}\\
\end{align*}

\newcommand{\dLogz}{-y_i w \exp(-y_i(w\tr x_i + b))}
\newcommand{\dLogn}{\zLog}


\begin{align*}
\frac{\partial}{\partial x \partial x} f_3(x) &= \frac{\partial}{\partial x}\left[ c \cdot \sum\limits_{i=1}^k \frac{\dLogz}{\dLogn}  \right] \\
&= c \cdot \sum\limits_{i=1}^k \frac{\partial}{\partial x} \left[  \frac{\dLogz}{\dLogn}  \right] = c \cdot \sum\limits_{i=1}^k \frac{ \frac{\partial}{\partial x} u(x_i) \cdot v(x_i) - u(x_i) \cdot \frac{\partial}{\partial x_i} v(x_i)} {v(x_i)^2}\\
\end{align*}





\begin{align*}
u(x) &= \dLogz\\
v(x) &= \dLogn\\
\frac{\partial}{\partial x} u(x) &= \frac{\partial}{\partial x} \left[\dLogz \right]\\
 &= -y_i w \exp(-y_i(w\tr x_i + b)) \frac{\partial}{\partial x} \left[ -y_i(w\tr x_i + b) \right] \\
&= y_i^2 w^2 \exp(-y_i(w\tr x_i + b)) \\  
\frac{\partial}{\partial x}  v(x) &= \frac{\partial}{\partial x} \left[  \dLogn \right] \\ 
&= \frac{\partial}{\partial x} \left[\exp(-y_i\left(w\tr x_i + b \right)) \right] \\ 
&= u(x)
\end{align*}

\begin{align*}
\frac{\partial}{\partial x \partial x} f_3(x) &= \frac{ y_i^2 w^2 \exp(-y_i(w\tr x_i + b)) \cdot \left(\dLogn\right) - \left( \dLogz \right)^2 } {\left(\dLogn\right)^2}\\
\end{align*}



%&\text{with } u(x) = \dLogz \text{ and } v(x) = \dLogn \\
%u





%&= c \cdot \sum\limits_{i=1}^k \frac{\frac{\partial}{\partial x} \left[ \dLogz \right] \cdot \dLogn - \dLogz \cdot \frac{\partial}{\partial x} \left[ \dLogn \right] } {\dLogn^2}
%\end{align*}
\end{document}
